prove correctness of exception handlers invoked from user-mode
ARMdef: split evalMOVSPCLRUC into a helper evalUserExecution without quantifiers

entry.i:
 * simplify lemma_userExecutionModel_validity to cover only the
   evalUserExecution part, not the continuation

 * lemma_userExecutionModel_validity also ensures
   userExecutionPreconditions, for convenience

 * simplify user entry preconditions to explicitly pass the dispPg

exception_handlers.sdfy:
 * simplify preconditions on interrupt_handler

main.dfy:
 * prove that whenever we take an exception from user mode, the
   handler's preconditions are satisfied and that it establishes the
   postcondition

(the last missing piece in the puzzle is an interrupt taken from
privileged modes)

verified/ARMdef.dfy
@@ -1172,17 +1172,22 @@ predicate evalCPSID_IAF(s:state, mod:word, r:state)
     && evalUpdate(s, OSReg(cpsr), newpsr, r)
 }
 
+predicate evalUserExecution(s:state, s2:state, s4:state)
+    requires ValidState(s) && ExtractAbsPageTable(s).Just?
+{
+    evalEnterUserspace(s, s2)
+    && var (s3, pc, ex) := userspaceExecutionFn(s2, OperandContents(s, OLR));
+       evalExceptionTaken(s3, ex, pc, s4)
+}
+
 predicate {:opaque} evalMOVSPCLRUC(s:state, r:state)
     requires ValidState(s)
     ensures evalMOVSPCLRUC(s, r) ==> ValidState(r)
 {
     ExtractAbsPageTable(s).Just?
     && UsermodeContinuationPrecondition(s)
-    && exists s2, s4 ::
-        evalEnterUserspace(s, s2)
-        && (var (s3, pc, ex) := userspaceExecutionFn(s2, OperandContents(s, OLR));
-        evalExceptionTaken(s3, ex, pc, s4)
-        && UsermodeContinuationInvariant(s4, r))
+    && exists s2, s4 :: evalUserExecution(s, s2, s4)
+    && UsermodeContinuationInvariant(s4, r)
 }
 
 predicate evalBlock(block:codes, s:state, r:state)
