verified/main.dfy
@@ -113,8 +113,17 @@ method printAll()
     printFooter();
 }
 
+// these are global assumptions
+predicate GlobalAssumptions()
+{
+    SaneConstants()
+        && UsermodeContinuationPreconditionDef()
+        && UsermodeContinuationInvariantDef()
+        && InterruptContinuationInvariantDef()
+}
+
 // this is what we assume about the initial state on entry to the SMC handler
-predicate InitialState(s:state)
+predicate InitialSMCState(s:state)
 {
     reveal_ValidRegState();
     reveal_ValidSRegState();
@@ -128,15 +137,128 @@ predicate InitialState(s:state)
         && decode_psr(s.sregs[spsr(Monitor)]).m != Monitor
 }
 
+function exHandler(ex:exception): va_code
+{
+    match ex
+        case ExAbt => abt_handler()
+        case ExUnd => und_handler()
+        case ExSVC => svc_handler()
+        case ExFIQ => fiq_handler()
+        case ExIRQ => irq_handler()
+}
+
+lemma lemma_KomUserEntryPrecond_AbsPT(s:state, pagedb:PageDb, dispPg:PageNr)
+    requires KomUserEntryPrecondition(s, pagedb, dispPg)
+    ensures ExtractAbsPageTable(s).Just?
+{
+    lemma_ptablesmatch(s.m, pagedb, l1pOfDispatcher(pagedb, dispPg));
+}
+
+predicate ExceptionStateSideEffects(s:state)
+{
+    if s.conf.ex == ExFIQ || s.conf.ex == ExIRQ
+        then mode_of_state(s) == Monitor && !interrupts_enabled(s)
+    else
+        spsr_of_state(s).m == User
+        && mode_of_state(s) == (match s.conf.ex
+            case ExAbt => Abort
+            case ExUnd => Undefined
+            case ExSVC => Supervisor)
+}
+
+lemma lemma_KomUserEntryPrecond_Preserved(s0:state, s2:state, r:state,
+                                          pagedb0:PageDb, dispPg:PageNr)
+                                          returns (pagedb: PageDb)
+    requires KomUserEntryPrecondition(s0, pagedb0, dispPg)
+    requires (lemma_KomUserEntryPrecond_AbsPT(s0, pagedb0, dispPg);
+              evalUserExecution(s0, s2, r))
+    ensures pagedb == updateUserPagesFromState(r, pagedb0, dispPg)
+    ensures KomUserEntryPrecondition(r, pagedb, dispPg)
+{
+    lemma_KomUserEntryPrecond_AbsPT(s0, pagedb0, dispPg);
+    lemma_userExecutionModel_validity(s0, s2, r);
+    lemma_userExecutionPreservesPrivState(s0, r);
+    lemma_userExecutionUpdatesPageDb(pagedb0, s0, r, dispPg);
+
+    pagedb := updateUserPagesFromState(r, pagedb0, dispPg);
+    assert l1pOfDispatcher(pagedb, dispPg) == l1pOfDispatcher(pagedb0, dispPg)
+        by { reveal updateUserPagesFromState(); }
+}
+
+lemma lemma_ExceptionStateSideEffects(s0:state, s2:state, r:state,
+                                      pagedb0:PageDb, dispPg:PageNr)
+    requires KomUserEntryPrecondition(s0, pagedb0, dispPg)
+    requires (lemma_KomUserEntryPrecond_AbsPT(s0, pagedb0, dispPg);
+              evalUserExecution(s0, s2, r))
+    ensures ExceptionStateSideEffects(r)
+{
+    lemma_KomUserEntryPrecond_AbsPT(s0, pagedb0, dispPg);
+    assert evalEnterUserspace(s0, s2);
+    assert mode_of_state(s2) == User;
+    lemma_evalEnterUserspace_preservesAbsPageTable(s0, s2);
+
+    var (s3, expc, ex) := userspaceExecutionFn(s2, OperandContents(s0, OLR));
+    assert mode_of_state(s3) == mode_of_state(s2) == User
+        && s3.conf.scr == s2.conf.scr == s0.conf.scr == SCRT(Secure, true, true)
+        by { reveal userspaceExecutionFn(); }
+
+    assert evalExceptionTaken(s3, ex, expc, r);
+    assert r.conf.ex == ex;
+    lemma_evalExceptionTaken_Mode(s3, ex, expc, r);
+    assert spsr_of_state(r).m == mode_of_state(s3) == User;
+    if ex == ExFIQ || ex == ExIRQ {
+        assert mode_of_state(r) == Monitor;
+        mode_encodings_are_sane();
+        lemma_update_psr(cpsr_of_state(s3), encode_mode(Monitor), true, true);
+        assert !interrupts_enabled(r);
+    }
+    assert ExceptionStateSideEffects(r);
+}
+
+lemma lemma_evalHandler(s:state, r:state, pagedb:PageDb, dispPg: PageNr)
+    requires GlobalAssumptions() && ExceptionStateSideEffects(s)
+    requires KomUserEntryPrecondition(s, pagedb, dispPg) && mode_of_state(s) != User
+    requires evalCode(exHandler(s.conf.ex), s, r)
+    requires spsr_of_state(s).m == User // proofs about PL1 interrupts go elsewhere
+    ensures KomExceptionHandlerInvariant(s, pagedb, r, dispPg)
+{
+    var block := va_CCons(exHandler(s.conf.ex), va_CNil());
+    reveal_va_eval();
+    assert va_eval(Block(block), s, r) by { assert evalBlock(block, s, r); }
+    if s.conf.ex == ExIRQ || s.conf.ex == ExFIQ {
+        var _, _, p := va_lemma_interrupt_handler(block, s, r, s.conf.ex, pagedb, dispPg);
+    } else if s.conf.ex == ExAbt || s.conf.ex == ExUnd {
+        var _, _, p := va_lemma_abort_handler(block, s, r, s.conf.ex, pagedb, dispPg);
+    } else if s.conf.ex == ExSVC {
+        var _, _, p := va_lemma_svc_handler(block, s, r, pagedb, dispPg);
+    }
+}
+
 method Main()
 {
-    // prove that the final state for an SMC call is valid
+    // prove that whenever we take an exception from user mode, we can run the right
+    // handler and it will establish the invariants assumed in the SMC path
+    forall s0:state, s1:state, s3:state, r:state
+        | GlobalAssumptions() && ValidState(s0) && s0.ok
+        && UsermodeContinuationPrecondition(s0)
+        && evalUserExecution(s0, s1, s3)
+        && evalCode(exHandler(s3.conf.ex), s3, r)
+        ensures exists p2, dp :: KomExceptionHandlerInvariant(s3, p2, r, dp)
+    {
+        var pagedb, dispPg := lemma_UsermodeContinuationPreconditionDef(s0);
+        assert KomUserEntryPrecondition(s0, pagedb, dispPg);
+        pagedb := lemma_KomUserEntryPrecond_Preserved(s0, s1, s3, pagedb, dispPg);
+        lemma_ExceptionStateSideEffects(s0, s1, s3, pagedb, dispPg);
+        lemma_evalHandler(s3, r, pagedb, dispPg);
+    }
+
+    // TODO: prove something about interrupts from PL1 modes
+    
+    // prove that the SMC handler is correct
     forall s1:state, p1:PageDb, s2:state
-        | InitialState(s1)
-        && validPageDb(p1)
-        && pageDbCorresponds(s1.m, p1)
+        | GlobalAssumptions() && InitialSMCState(s1)
+        && validPageDb(p1) && pageDbCorresponds(s1.m, p1)
         && evalCode(smc_handler(), s1, s2)
-        && UsermodeContinuationInvariantDef() // XXX
         ensures exists p2:PageDb :: smchandler(s1, p1, s2, p2)
             && validPageDb(p2) && pageDbCorresponds(s2.m, p2)
     {
@@ -149,5 +271,6 @@ method Main()
         assert smchandler(s1, p1, s2, p2');
         assert validPageDb(p2') && pageDbCorresponds(s2.m, p2');
     }
+
     printAll();
 }
